cfrontend/Cstrategy.v
@@ -1909,7 +1909,7 @@ with eval_funcall: compartment -> mem -> fundef -> list val -> trace -> mem -> v
   | eval_funcall_internal: forall cp m f vargs t e m1 m2 m3 out vres m4,
       list_norepet (var_names f.(fn_params) ++ var_names f.(fn_vars)) ->
       alloc_variables ge empty_env m (f.(fn_params) ++ f.(fn_vars)) e m1 ->
-      bind_parameters ge e cp m1 f.(fn_params) vargs m2 ->
+      bind_parameters ge e (comp_of f) m1 f.(fn_params) vargs m2 ->
       exec_stmt f.(fn_comp) e m2 f.(fn_body) t m3 out ->
       outcome_result_value out f.(fn_return) vres m3 ->
       Mem.free_list m3 (blocks_of_env ge e) f.(fn_comp) = Some m4 ->
@@ -2132,7 +2132,7 @@ with evalinf_funcall: compartment -> mem -> fundef -> list val -> traceinf -> Pr
   | evalinf_funcall_internal: forall cp m f vargs t e m1 m2,
       list_norepet (var_names f.(fn_params) ++ var_names f.(fn_vars)) ->
       alloc_variables ge empty_env m (f.(fn_params) ++ f.(fn_vars)) e m1 ->
-      bind_parameters ge e cp m1 f.(fn_params) vargs m2 ->
+      bind_parameters ge e (comp_of f) m1 f.(fn_params) vargs m2 ->
       execinf_stmt f.(fn_comp) e m2 f.(fn_body) t ->
       evalinf_funcall cp m (Internal f) vargs t.
 
